coq/src/ConcordiumImpls_template.v
@@ -5,6 +5,8 @@ Import List.ListNotations.
 Open Scope Z_scope.
 Open Scope bool_scope.
 Open Scope hacspec_scope.
+From QuickChick Require Import QuickChick.
+Require Import QuickChickLib.
 Require Import Hacspec.Lib.
 
 Notation "'reject_hacspec_t'" := (int32) : hacspec_scope.
@@ -21,26 +23,29 @@ Definition reject_impl_convert_from_unit  : reject_hacspec_t :=
 
 Theorem ensures_reject_impl_convert_from_unit : forall result_1 ,
 @reject_impl_convert_from_unit  = result_1 ->
-(result_1) !=.? (@repr WORDSIZE32 0).
-Proof.
-  intros ; subst.
-  reflexivity.
-Qed.
+~ (result_1 = @repr WORDSIZE32 0).
+Proof. Admitted.
 
 Definition reject_impl_convert_from_parse_error  : reject_hacspec_t :=
   (min_v) .+ (@repr WORDSIZE32 2).
 
 Theorem ensures_reject_impl_convert_from_parse_error : forall result_1 ,
 @reject_impl_convert_from_parse_error  = result_1 ->
-(result_1) !=.? (@repr WORDSIZE32 0).
-Proof.
-  intros ; subst.
-  reflexivity.
-Qed.
+~ (result_1 = @repr WORDSIZE32 0).
+Proof. Admitted.
 
 Inductive log_error_t :=
 | Full : log_error_t
 | Malformed : log_error_t.
+Global Instance show_log_error_t : Show (log_error_t) :=
+ @Build_Show (log_error_t) (fun x =>
+ match x with
+ Full => ("Full")%string
+ | Malformed => ("Malformed")%string
+ end).
+Definition g_log_error_t : G (log_error_t) := oneOf_ (returnGen Full) [returnGen Full;returnGen Malformed].
+Global Instance gen_log_error_t : Gen (log_error_t) := Build_Gen log_error_t g_log_error_t.
+
 
 Definition reject_impl_from_log_error (le_2 : log_error_t) : reject_hacspec_t :=
   match le_2 with
@@ -51,17 +56,27 @@ Definition reject_impl_from_log_error (le_2 : log_error_t) : reject_hacspec_t :=
 Theorem ensures_reject_impl_from_log_error : forall result_1 (
   le_2 : log_error_t),
 @reject_impl_from_log_error le_2 = result_1 ->
-(result_1) !=.? (@repr WORDSIZE32 0).
-Proof.
-  intros ; subst.
-  destruct le_2 ; reflexivity.
-Qed.
+~ (result_1 = @repr WORDSIZE32 0).
+Proof. Admitted.
 
 Inductive new_contract_name_error_t :=
 | NewContractNameErrorMissingInitPrefix : new_contract_name_error_t
 | NewContractNameErrorTooLong : new_contract_name_error_t
 | NewContractNameErrorContainsDot : new_contract_name_error_t
 | NewContractNameErrorInvalidCharacters : new_contract_name_error_t.
+Global Instance show_new_contract_name_error_t : Show (new_contract_name_error_t) :=
+ @Build_Show (new_contract_name_error_t) (fun x =>
+ match x with
+ NewContractNameErrorMissingInitPrefix => (
+   "NewContractNameErrorMissingInitPrefix")%string
+ | NewContractNameErrorTooLong => ("NewContractNameErrorTooLong")%string
+ | NewContractNameErrorContainsDot => ("NewContractNameErrorContainsDot")%string
+ | NewContractNameErrorInvalidCharacters => (
+   "NewContractNameErrorInvalidCharacters")%string
+ end).
+Definition g_new_contract_name_error_t : G (new_contract_name_error_t) := oneOf_ (returnGen NewContractNameErrorMissingInitPrefix) [returnGen NewContractNameErrorMissingInitPrefix;returnGen NewContractNameErrorTooLong;returnGen NewContractNameErrorContainsDot;returnGen NewContractNameErrorInvalidCharacters].
+Global Instance gen_new_contract_name_error_t : Gen (new_contract_name_error_t) := Build_Gen new_contract_name_error_t g_new_contract_name_error_t.
+
 
 Definition reject_impl_from_new_contract_name_error
   (nre_3 : new_contract_name_error_t)
@@ -76,16 +91,25 @@ Definition reject_impl_from_new_contract_name_error
 Theorem ensures_reject_impl_from_new_contract_name_error : forall result_1 (
   nre_3 : new_contract_name_error_t),
 @reject_impl_from_new_contract_name_error nre_3 = result_1 ->
-(result_1) !=.? (@repr WORDSIZE32 0).
-Proof.
-  intros ; subst.
-  destruct nre_3 ; reflexivity.
-Qed.
+~ (result_1 = @repr WORDSIZE32 0).
+Proof. Admitted.
 
 Inductive new_receive_name_error_t :=
 | NewReceiveNameErrorMissingDotSeparator : new_receive_name_error_t
 | NewReceiveNameErrorTooLong : new_receive_name_error_t
 | NewReceiveNameErrorInvalidCharacters : new_receive_name_error_t.
+Global Instance show_new_receive_name_error_t : Show (new_receive_name_error_t) :=
+ @Build_Show (new_receive_name_error_t) (fun x =>
+ match x with
+ NewReceiveNameErrorMissingDotSeparator => (
+   "NewReceiveNameErrorMissingDotSeparator")%string
+ | NewReceiveNameErrorTooLong => ("NewReceiveNameErrorTooLong")%string
+ | NewReceiveNameErrorInvalidCharacters => (
+   "NewReceiveNameErrorInvalidCharacters")%string
+ end).
+Definition g_new_receive_name_error_t : G (new_receive_name_error_t) := oneOf_ (returnGen NewReceiveNameErrorMissingDotSeparator) [returnGen NewReceiveNameErrorMissingDotSeparator;returnGen NewReceiveNameErrorTooLong;returnGen NewReceiveNameErrorInvalidCharacters].
+Global Instance gen_new_receive_name_error_t : Gen (new_receive_name_error_t) := Build_Gen new_receive_name_error_t g_new_receive_name_error_t.
+
 
 Definition reject_impl_from_new_receive_name_error
   (nre_4 : new_receive_name_error_t)
@@ -99,11 +123,8 @@ Definition reject_impl_from_new_receive_name_error
 Theorem ensures_reject_impl_from_new_receive_name_error : forall result_1 (
   nre_4 : new_receive_name_error_t),
 @reject_impl_from_new_receive_name_error nre_4 = result_1 ->
-(result_1) !=.? (@repr WORDSIZE32 0).
-Proof.
-  intros ; subst.
-  destruct nre_4 ; reflexivity.
-Qed.
+~ (result_1 = @repr WORDSIZE32 0).
+Proof. Admitted.
 
 Notation "'contract_state_hacspec_t'" := (int32) : hacspec_scope.
 
@@ -111,6 +132,16 @@ Inductive seek_from_t :=
 | Start : int64 -> seek_from_t
 | End : int64 -> seek_from_t
 | Current : int64 -> seek_from_t.
+Global Instance show_seek_from_t : Show (seek_from_t) :=
+ @Build_Show (seek_from_t) (fun x =>
+ match x with
+ Start a => ("Start" ++ show a)%string
+ | End a => ("End" ++ show a)%string
+ | Current a => ("Current" ++ show a)%string
+ end).
+Definition g_seek_from_t : G (seek_from_t) := oneOf_ (bindGen arbitrary (fun a => returnGen (Start a))) [bindGen arbitrary (fun a => returnGen (Start a));bindGen arbitrary (fun a => returnGen (End a));bindGen arbitrary (fun a => returnGen (Current a))].
+Global Instance gen_seek_from_t : Gen (seek_from_t) := Build_Gen seek_from_t g_seek_from_t.
+
 
 Notation "'uint32_option_t'" := ((option int32)) : hacspec_scope.
 
@@ -291,6 +322,16 @@ Definition get_policy_section_hacspec
   (policy_bytes_52, @repr WORDSIZE32 1).
 
 Notation "'attributes_cursor_hacspec_t'" := ((int32 × int16)) : hacspec_scope.
+Instance show_attributes_cursor_hacspec_t : Show (attributes_cursor_hacspec_t) :=
+Build_Show attributes_cursor_hacspec_t (fun x =>
+  let (x, x0) := x in
+  (("(") ++ ((show x) ++ ((",") ++ ((show x0) ++ (")"))))))%string.
+Definition g_attributes_cursor_hacspec_t : G (attributes_cursor_hacspec_t) :=
+bindGen arbitrary (fun x0 : int32 =>
+  bindGen arbitrary (fun x1 : int16 =>
+  returnGen (x0,x1))).
+Instance gen_attributes_cursor_hacspec_t : Gen (attributes_cursor_hacspec_t) := Build_Gen attributes_cursor_hacspec_t g_attributes_cursor_hacspec_t.
+
 
 Definition has_policy_impl_for_policy_attributes_cursor_next_item
   (policy_attribute_items_54 : attributes_cursor_hacspec_t)
@@ -326,6 +367,16 @@ Definition has_policy_impl_for_policy_attributes_cursor_next_item
     )))).
 
 Notation "'policies_iterator_hacspec_t'" := ((int32 × int16)) : hacspec_scope.
+Instance show_policies_iterator_hacspec_t : Show (policies_iterator_hacspec_t) :=
+Build_Show policies_iterator_hacspec_t (fun x =>
+  let (x, x0) := x in
+  (("(") ++ ((show x) ++ ((",") ++ ((show x0) ++ (")"))))))%string.
+Definition g_policies_iterator_hacspec_t : G (policies_iterator_hacspec_t) :=
+bindGen arbitrary (fun x0 : int32 =>
+  bindGen arbitrary (fun x1 : int16 =>
+  returnGen (x0,x1))).
+Instance gen_policies_iterator_hacspec_t : Gen (policies_iterator_hacspec_t) := Build_Gen policies_iterator_hacspec_t g_policies_iterator_hacspec_t.
+
 
 Notation "'policy_attributes_cursor_hacspec_t'" := ((
   int32 ×
@@ -333,6 +384,21 @@ Notation "'policy_attributes_cursor_hacspec_t'" := ((
   int64 ×
   attributes_cursor_hacspec_t
 )) : hacspec_scope.
+Instance show_policy_attributes_cursor_hacspec_t : Show (policy_attributes_cursor_hacspec_t) :=
+Build_Show policy_attributes_cursor_hacspec_t (fun x =>
+  let (x, x0) := x in
+  let (x, x1) := x in
+  let (x, x2) := x in
+  (
+    ("(") ++ ((show x) ++ ((",") ++ ((show x0) ++ ((",") ++ ((show x1) ++ ((",") ++ ((show x2) ++ (")"))))))))))%string.
+Definition g_policy_attributes_cursor_hacspec_t : G (policy_attributes_cursor_hacspec_t) :=
+bindGen arbitrary (fun x0 : int32 =>
+  bindGen arbitrary (fun x1 : int64 =>
+  bindGen arbitrary (fun x2 : int64 =>
+  bindGen arbitrary (fun x3 : attributes_cursor_hacspec_t =>
+  returnGen (x0,x1,x2,x3))))).
+Instance gen_policy_attributes_cursor_hacspec_t : Gen (policy_attributes_cursor_hacspec_t) := Build_Gen policy_attributes_cursor_hacspec_t g_policy_attributes_cursor_hacspec_t.
+
 
 Definition iterator_impl_for_policies_iterator_next
   (policies_iterator_62 : policies_iterator_hacspec_t)
@@ -451,3 +517,754 @@ Definition combine_and_hacspec (l_89 : int32) (r_90 : int32) : int32 :=
 
 Definition combine_or_hacspec (l_91 : int32) (r_92 : int32) : int32 :=
   @repr WORDSIZE32 1.
+
+Definition user_address_t := nseq (int8) (usize 32).
+
+Inductive auction_state_t :=
+| NotSoldYet : auction_state_t
+| Sold : user_address_t -> auction_state_t.
+
+Definition eqb_auction_state_t (x y : auction_state_t) : bool :=
+match x with
+   | NotSoldYet => match y with | NotSoldYet=> true | _ => false end
+   | Sold a => match y with | Sold b => a =.? b | _ => false end
+   end.
+
+Definition eqb_leibniz_auction_state_t (x y : auction_state_t) : eqb_auction_state_t x y = true <-> x = y.
+Proof. split. intros; destruct x ; destruct y ; try (f_equal ; apply eqb_leibniz) ; easy. intros ; subst ; destruct y ; try reflexivity ; try (apply eqb_refl). Qed.
+
+Instance eq_dec_auction_state_t : EqDec (auction_state_t) :=
+Build_EqDec (auction_state_t) (eqb_auction_state_t) (eqb_leibniz_auction_state_t).
+
+Global Instance show_auction_state_t : Show (auction_state_t) :=
+ @Build_Show (auction_state_t) (fun x =>
+ match x with
+ NotSoldYet => ("NotSoldYet")%string
+ | Sold a => ("Sold" ++ show a)%string
+ end).
+Definition g_auction_state_t : G (auction_state_t) := oneOf_ (returnGen NotSoldYet) [returnGen NotSoldYet;bindGen arbitrary (fun a => returnGen (Sold a))].
+Global Instance gen_auction_state_t : Gen (auction_state_t) := Build_Gen auction_state_t g_auction_state_t.
+
+
+Inductive seq_map_t :=
+| SeqMap : (public_byte_seq × public_byte_seq) -> seq_map_t.
+
+Definition eqb_seq_map_t (x y : seq_map_t) : bool :=
+match x with
+   | SeqMap a => match y with | SeqMap b => a =.? b end
+   end.
+
+Definition eqb_leibniz_seq_map_t (x y : seq_map_t) : eqb_seq_map_t x y = true <-> x = y.
+Proof. split. intros; destruct x ; destruct y ; try (f_equal ; apply eqb_leibniz) ; easy. intros ; subst ; destruct y ; try reflexivity ; try (apply eqb_refl). Qed.
+
+Instance eq_dec_seq_map_t : EqDec (seq_map_t) :=
+Build_EqDec (seq_map_t) (eqb_seq_map_t) (eqb_leibniz_seq_map_t).
+
+Global Instance show_seq_map_t : Show (seq_map_t) :=
+ @Build_Show (seq_map_t) (fun x =>
+ match x with
+ SeqMap a => ("SeqMap" ++ show a)%string
+ end).
+Definition g_seq_map_t : G (seq_map_t) := oneOf_ (bindGen arbitrary (fun a => returnGen (SeqMap a))) [bindGen arbitrary (fun a => returnGen (SeqMap a))].
+Global Instance gen_seq_map_t : Gen (seq_map_t) := Build_Gen seq_map_t g_seq_map_t.
+
+
+Notation "'amount_hacspec_t'" := (int64) : hacspec_scope.
+
+Notation "'timestamp_hacspec_t'" := (int64) : hacspec_scope.
+
+Notation "'itemtyp_t'" := (public_byte_seq) : hacspec_scope.
+
+Inductive state_t :=
+| State : (
+  auction_state_t ×
+  amount_hacspec_t ×
+  itemtyp_t ×
+  timestamp_hacspec_t ×
+  seq_map_t
+) -> state_t.
+
+Definition eqb_state_t (x y : state_t) : bool :=
+match x with
+   | State a => match y with | State b => a =.? b end
+   end.
+
+Definition eqb_leibniz_state_t (x y : state_t) : eqb_state_t x y = true <-> x = y.
+Proof. split. intros; destruct x ; destruct y ; try (f_equal ; apply eqb_leibniz) ; easy. intros ; subst ; destruct y ; try reflexivity ; try (apply eqb_refl). Qed.
+
+Instance eq_dec_state_t : EqDec (state_t) :=
+Build_EqDec (state_t) (eqb_state_t) (eqb_leibniz_state_t).
+
+Global Instance show_state_t : Show (state_t) :=
+ @Build_Show (state_t) (fun x =>
+ match x with
+ State a => ("State" ++ show a)%string
+ end).
+Definition g_state_t : G (state_t) := oneOf_ (bindGen arbitrary (fun a => returnGen (State a))) [bindGen arbitrary (fun a => returnGen (State a))].
+Global Instance gen_state_t : Gen (state_t) := Build_Gen state_t g_state_t.
+
+
+Definition fresh_state (itm_93 : itemtyp_t) (exp_94 : int64) : state_t :=
+  State ((
+      NotSoldYet,
+      @repr WORDSIZE64 0,
+      itm_93,
+      exp_94,
+      SeqMap ((seq_new_ (default) (usize 0), seq_new_ (default) (usize 0)))
+    )).
+
+Theorem ensures_fresh_state : forall result_1 (itm_93 : itemtyp_t) (
+  exp_94 : int64),
+@fresh_state itm_93 exp_94 = result_1 ->
+true.
+Proof. Admitted.
+
+Definition seq_map_entry
+  (m_95 : seq_map_t)
+  (sender_address_96 : user_address_t)
+  : (int64 × seq_map_t) :=
+  let 'SeqMap ((m0_97, m1_98)) :=
+    m_95 in 
+  let res_99 : (int64 × seq_map_t) :=
+    (
+      @repr WORDSIZE64 0,
+      SeqMap ((
+          seq_concat ((m0_97)) (sender_address_96),
+          seq_concat ((m1_98)) (u64_to_be_bytes (@repr WORDSIZE64 0))
+        ))
+    ) in 
+  let res_99 :=
+    foldi (usize 0) ((seq_len ((m0_97))) / (usize 32)) (fun x_100 res_99 =>
+      let '(res_99) :=
+        if (array_from_seq (32) (seq_slice ((m0_97)) ((x_100) * (usize 32)) (
+              usize 32))) array_eq (sender_address_96):bool then (let res_99 :=
+            (
+              u64_from_be_bytes (array_from_seq (8) (seq_slice ((m1_98)) ((
+                      x_100) * (usize 8)) (usize 8))),
+              SeqMap (((m0_97), (m1_98)))
+            ) in 
+          (res_99)) else ((res_99)) in 
+      (res_99))
+    res_99 in 
+  res_99.
+
+Inductive map_update_t :=
+| Update : (int64 × seq_map_t) -> map_update_t.
+
+Definition eqb_map_update_t (x y : map_update_t) : bool :=
+match x with
+   | Update a => match y with | Update b => a =.? b end
+   end.
+
+Definition eqb_leibniz_map_update_t (x y : map_update_t) : eqb_map_update_t x y = true <-> x = y.
+Proof. split. intros; destruct x ; destruct y ; try (f_equal ; apply eqb_leibniz) ; easy. intros ; subst ; destruct y ; try reflexivity ; try (apply eqb_refl). Qed.
+
+Instance eq_dec_map_update_t : EqDec (map_update_t) :=
+Build_EqDec (map_update_t) (eqb_map_update_t) (eqb_leibniz_map_update_t).
+
+Global Instance show_map_update_t : Show (map_update_t) :=
+ @Build_Show (map_update_t) (fun x =>
+ match x with
+ Update a => ("Update" ++ show a)%string
+ end).
+Definition g_map_update_t : G (map_update_t) := oneOf_ (bindGen arbitrary (fun a => returnGen (Update a))) [bindGen arbitrary (fun a => returnGen (Update a))].
+Global Instance gen_map_update_t : Gen (map_update_t) := Build_Gen map_update_t g_map_update_t.
+
+
+Definition seq_map_update_entry
+  (m_101 : seq_map_t)
+  (sender_address_102 : user_address_t)
+  (amount_103 : int64)
+  : map_update_t :=
+  let 'SeqMap ((m0_104, m1_105)) :=
+    m_101 in 
+  let res_106 : map_update_t :=
+    Update ((
+        amount_103,
+        SeqMap ((
+            seq_concat ((m0_104)) (sender_address_102),
+            seq_concat ((m1_105)) (u64_to_be_bytes (amount_103))
+          ))
+      )) in 
+  let res_106 :=
+    foldi (usize 0) ((seq_len ((m0_104))) / (usize 32)) (fun x_107 res_106 =>
+      let '(res_106) :=
+        if (array_from_seq (32) (seq_slice ((m0_104)) ((x_107) * (usize 32)) (
+              usize 32))) array_eq (sender_address_102):bool then (
+          let res_106 :=
+            Update ((
+                amount_103,
+                SeqMap ((
+                    seq_update ((m0_104)) ((x_107) * (usize 32)) (
+                      sender_address_102),
+                    seq_update ((m1_105)) ((x_107) * (usize 8)) (
+                      u64_to_be_bytes (amount_103))
+                  ))
+              )) in 
+          (res_106)) else ((res_106)) in 
+      (res_106))
+    res_106 in 
+  res_106.
+
+Inductive bid_error_t :=
+| ContractSender : bid_error_t
+| BidTooLow : bid_error_t
+| BidsOverWaitingForAuctionFinalization : bid_error_t
+| AuctionIsFinalized : bid_error_t.
+
+Definition eqb_bid_error_t (x y : bid_error_t) : bool :=
+match x with
+   | ContractSender => match y with | ContractSender=> true | _ => false end
+   | BidTooLow => match y with | BidTooLow=> true | _ => false end
+   | BidsOverWaitingForAuctionFinalization =>
+       match y with
+       | BidsOverWaitingForAuctionFinalization=> true
+       | _ => false
+       end
+   | AuctionIsFinalized =>
+       match y with
+       | AuctionIsFinalized=> true
+       | _ => false
+       end
+   end.
+
+Definition eqb_leibniz_bid_error_t (x y : bid_error_t) : eqb_bid_error_t x y = true <-> x = y.
+Proof. split. intros; destruct x ; destruct y ; try (f_equal ; apply eqb_leibniz) ; easy. intros ; subst ; destruct y ; try reflexivity ; try (apply eqb_refl). Qed.
+
+Instance eq_dec_bid_error_t : EqDec (bid_error_t) :=
+Build_EqDec (bid_error_t) (eqb_bid_error_t) (eqb_leibniz_bid_error_t).
+
+Global Instance show_bid_error_t : Show (bid_error_t) :=
+ @Build_Show (bid_error_t) (fun x =>
+ match x with
+ ContractSender => ("ContractSender")%string
+ | BidTooLow => ("BidTooLow")%string
+ | BidsOverWaitingForAuctionFinalization => (
+   "BidsOverWaitingForAuctionFinalization")%string
+ | AuctionIsFinalized => ("AuctionIsFinalized")%string
+ end).
+Definition g_bid_error_t : G (bid_error_t) := oneOf_ (returnGen ContractSender) [returnGen ContractSender;returnGen BidTooLow;returnGen BidsOverWaitingForAuctionFinalization;returnGen AuctionIsFinalized].
+Global Instance gen_bid_error_t : Gen (bid_error_t) := Build_Gen bid_error_t g_bid_error_t.
+
+
+Inductive user_address_set_t :=
+| UserAddressSome : user_address_t -> user_address_set_t
+| UserAddressNone : user_address_set_t.
+
+Definition eqb_user_address_set_t (x y : user_address_set_t) : bool :=
+match x with
+   | UserAddressSome a =>
+       match y with
+       | UserAddressSome b => a =.? b
+       | _ => false
+       end
+   | UserAddressNone => match y with | UserAddressNone=> true | _ => false end
+   end.
+
+Definition eqb_leibniz_user_address_set_t (x y : user_address_set_t) : eqb_user_address_set_t x y = true <-> x = y.
+Proof. split. intros; destruct x ; destruct y ; try (f_equal ; apply eqb_leibniz) ; easy. intros ; subst ; destruct y ; try reflexivity ; try (apply eqb_refl). Qed.
+
+Instance eq_dec_user_address_set_t : EqDec (user_address_set_t) :=
+Build_EqDec (user_address_set_t) (eqb_user_address_set_t) (eqb_leibniz_user_address_set_t).
+
+Global Instance show_user_address_set_t : Show (user_address_set_t) :=
+ @Build_Show (user_address_set_t) (fun x =>
+ match x with
+ UserAddressSome a => ("UserAddressSome" ++ show a)%string
+ | UserAddressNone => ("UserAddressNone")%string
+ end).
+Definition g_user_address_set_t : G (user_address_set_t) := oneOf_ (bindGen arbitrary (fun a => returnGen (UserAddressSome a))) [bindGen arbitrary (fun a => returnGen (UserAddressSome a));returnGen UserAddressNone].
+Global Instance gen_user_address_set_t : Gen (user_address_set_t) := Build_Gen user_address_set_t g_user_address_set_t.
+
+
+Notation "'context_t'" := ((int64 × user_address_set_t)) : hacspec_scope.
+Instance show_context_t : Show (context_t) :=
+Build_Show context_t (fun x =>
+  let (x, x0) := x in
+  (("(") ++ ((show x) ++ ((",") ++ ((show x0) ++ (")"))))))%string.
+Definition g_context_t : G (context_t) :=
+bindGen arbitrary (fun x0 : int64 =>
+  bindGen arbitrary (fun x1 : user_address_set_t =>
+  returnGen (x0,x1))).
+Instance gen_context_t : Gen (context_t) := Build_Gen context_t g_context_t.
+
+
+Notation "'auction_bid_result_t'" := ((
+  result state_t bid_error_t)) : hacspec_scope.
+
+Definition auction_bid
+  (ctx_108 : context_t)
+  (amount_109 : int64)
+  (state_110 : state_t)
+  : auction_bid_result_t :=
+  let 'State ((auction_state_111, highest_bid_112, st2_113, expiry_114, st4_115
+      )) :=
+    (state_110) in 
+  ifbnd negb ((auction_state_111) =.? (NotSoldYet)) : bool
+  thenbnd (bind (@Err state_t bid_error_t (AuctionIsFinalized)) (fun _ => Ok (
+        tt)))
+  else (tt) >> (fun 'tt =>
+  let '(slot_time_116, sender_117) :=
+    ctx_108 in 
+  ifbnd negb ((slot_time_116) <=.? (expiry_114)) : bool
+  thenbnd (bind (@Err state_t bid_error_t (
+        BidsOverWaitingForAuctionFinalization)) (fun _ => Ok (tt)))
+  else (tt) >> (fun 'tt =>
+  ifbnd (sender_117) =.? (UserAddressNone) : bool
+  thenbnd (bind (@Err state_t bid_error_t (ContractSender)) (fun _ => Ok (tt)))
+  else (tt) >> (fun 'tt =>
+  let sender_address_118 : user_address_t :=
+    match sender_117 with
+    | UserAddressNone => array_from_list int8 (let l :=
+        [
+          @repr WORDSIZE8 5;
+          @repr WORDSIZE8 5;
+          @repr WORDSIZE8 5;
+          @repr WORDSIZE8 5;
+          @repr WORDSIZE8 5;
+          @repr WORDSIZE8 5;
+          @repr WORDSIZE8 5;
+          @repr WORDSIZE8 5;
+          @repr WORDSIZE8 5;
+          @repr WORDSIZE8 5;
+          @repr WORDSIZE8 5;
+          @repr WORDSIZE8 5;
+          @repr WORDSIZE8 5;
+          @repr WORDSIZE8 5;
+          @repr WORDSIZE8 5;
+          @repr WORDSIZE8 5;
+          @repr WORDSIZE8 5;
+          @repr WORDSIZE8 5;
+          @repr WORDSIZE8 5;
+          @repr WORDSIZE8 5;
+          @repr WORDSIZE8 5;
+          @repr WORDSIZE8 5;
+          @repr WORDSIZE8 5;
+          @repr WORDSIZE8 5;
+          @repr WORDSIZE8 5;
+          @repr WORDSIZE8 5;
+          @repr WORDSIZE8 5;
+          @repr WORDSIZE8 5;
+          @repr WORDSIZE8 5;
+          @repr WORDSIZE8 5;
+          @repr WORDSIZE8 5;
+          @repr WORDSIZE8 5
+        ] in  l)
+    | UserAddressSome account_address_119 => account_address_119
+    end in 
+  let '(bid_to_update_120, new_map_121) :=
+    seq_map_entry ((st4_115)) (sender_address_118) in 
+  let '(updated_bid_122, updated_map_123) :=
+    match seq_map_update_entry ((st4_115)) (sender_address_118) ((
+        bid_to_update_120) .+ (amount_109)) with
+    | Update (updated_bid_124, updated_map_125) => (
+      updated_bid_124,
+      updated_map_125
+    )
+    end in 
+  ifbnd negb ((updated_bid_122) >.? (highest_bid_112)) : bool
+  thenbnd (bind (@Err state_t bid_error_t (BidTooLow)) (fun _ => Ok (tt)))
+  else (tt) >> (fun 'tt =>
+  @Ok state_t bid_error_t (State ((
+        auction_state_111,
+        updated_bid_122,
+        st2_113,
+        expiry_114,
+        updated_map_123
+      ))))))).
+
+Notation "'finalize_context_t'" := ((int64 × user_address_t × int64
+)) : hacspec_scope.
+Instance show_finalize_context_t : Show (finalize_context_t) :=
+Build_Show finalize_context_t (fun x =>
+  let (x, x0) := x in
+  let (x, x1) := x in
+  (
+    ("(") ++ ((show x) ++ ((",") ++ ((show x0) ++ ((",") ++ ((show x1) ++ (")"))))))))%string.
+Definition g_finalize_context_t : G (finalize_context_t) :=
+bindGen arbitrary (fun x0 : int64 =>
+  bindGen arbitrary (fun x1 : user_address_t =>
+  bindGen arbitrary (fun x2 : int64 =>
+  returnGen (x0,x1,x2)))).
+Instance gen_finalize_context_t : Gen (finalize_context_t) := Build_Gen finalize_context_t g_finalize_context_t.
+
+
+Inductive finalize_error_t :=
+| BidMapError : finalize_error_t
+| AuctionStillActive : finalize_error_t
+| AuctionFinalized : finalize_error_t.
+
+Definition eqb_finalize_error_t (x y : finalize_error_t) : bool :=
+match x with
+   | BidMapError => match y with | BidMapError=> true | _ => false end
+   | AuctionStillActive =>
+       match y with
+       | AuctionStillActive=> true
+       | _ => false
+       end
+   | AuctionFinalized => match y with | AuctionFinalized=> true | _ => false end
+   end.
+
+Definition eqb_leibniz_finalize_error_t (x y : finalize_error_t) : eqb_finalize_error_t x y = true <-> x = y.
+Proof. split. intros; destruct x ; destruct y ; try (f_equal ; apply eqb_leibniz) ; easy. intros ; subst ; destruct y ; try reflexivity ; try (apply eqb_refl). Qed.
+
+Instance eq_dec_finalize_error_t : EqDec (finalize_error_t) :=
+Build_EqDec (finalize_error_t) (eqb_finalize_error_t) (eqb_leibniz_finalize_error_t).
+
+Global Instance show_finalize_error_t : Show (finalize_error_t) :=
+ @Build_Show (finalize_error_t) (fun x =>
+ match x with
+ BidMapError => ("BidMapError")%string
+ | AuctionStillActive => ("AuctionStillActive")%string
+ | AuctionFinalized => ("AuctionFinalized")%string
+ end).
+Definition g_finalize_error_t : G (finalize_error_t) := oneOf_ (returnGen BidMapError) [returnGen BidMapError;returnGen AuctionStillActive;returnGen AuctionFinalized].
+Global Instance gen_finalize_error_t : Gen (finalize_error_t) := Build_Gen finalize_error_t g_finalize_error_t.
+
+
+Inductive finalize_action_t :=
+| Accept : finalize_action_t
+| SimpleTransfer : public_byte_seq -> finalize_action_t.
+
+Definition eqb_finalize_action_t (x y : finalize_action_t) : bool :=
+match x with
+   | Accept => match y with | Accept=> true | _ => false end
+   | SimpleTransfer a =>
+       match y with
+       | SimpleTransfer b => a =.? b
+       | _ => false
+       end
+   end.
+
+Definition eqb_leibniz_finalize_action_t (x y : finalize_action_t) : eqb_finalize_action_t x y = true <-> x = y.
+Proof. split. intros; destruct x ; destruct y ; try (f_equal ; apply eqb_leibniz) ; easy. intros ; subst ; destruct y ; try reflexivity ; try (apply eqb_refl). Qed.
+
+Instance eq_dec_finalize_action_t : EqDec (finalize_action_t) :=
+Build_EqDec (finalize_action_t) (eqb_finalize_action_t) (eqb_leibniz_finalize_action_t).
+
+Global Instance show_finalize_action_t : Show (finalize_action_t) :=
+ @Build_Show (finalize_action_t) (fun x =>
+ match x with
+ Accept => ("Accept")%string
+ | SimpleTransfer a => ("SimpleTransfer" ++ show a)%string
+ end).
+Definition g_finalize_action_t : G (finalize_action_t) := oneOf_ (returnGen Accept) [returnGen Accept;bindGen arbitrary (fun a => returnGen (SimpleTransfer a))].
+Global Instance gen_finalize_action_t : Gen (finalize_action_t) := Build_Gen finalize_action_t g_finalize_action_t.
+
+
+Inductive bid_remain_t :=
+| BidNone : bid_remain_t
+| BidSome : int64 -> bid_remain_t.
+
+Definition eqb_bid_remain_t (x y : bid_remain_t) : bool :=
+match x with
+   | BidNone => match y with | BidNone=> true | _ => false end
+   | BidSome a => match y with | BidSome b => a =.? b | _ => false end
+   end.
+
+Definition eqb_leibniz_bid_remain_t (x y : bid_remain_t) : eqb_bid_remain_t x y = true <-> x = y.
+Proof. split. intros; destruct x ; destruct y ; try (f_equal ; apply eqb_leibniz) ; easy. intros ; subst ; destruct y ; try reflexivity ; try (apply eqb_refl). Qed.
+
+Instance eq_dec_bid_remain_t : EqDec (bid_remain_t) :=
+Build_EqDec (bid_remain_t) (eqb_bid_remain_t) (eqb_leibniz_bid_remain_t).
+
+Global Instance show_bid_remain_t : Show (bid_remain_t) :=
+ @Build_Show (bid_remain_t) (fun x =>
+ match x with
+ BidNone => ("BidNone")%string
+ | BidSome a => ("BidSome" ++ show a)%string
+ end).
+Definition g_bid_remain_t : G (bid_remain_t) := oneOf_ (returnGen BidNone) [returnGen BidNone;bindGen arbitrary (fun a => returnGen (BidSome a))].
+Global Instance gen_bid_remain_t : Gen (bid_remain_t) := Build_Gen bid_remain_t g_bid_remain_t.
+
+
+Notation "'auction_finalize_result_t'" := ((result (state_t × finalize_action_t
+  ) finalize_error_t)) : hacspec_scope.
+
+Definition auction_finalize
+  (ctx_126 : finalize_context_t)
+  (state_127 : state_t)
+  : auction_finalize_result_t :=
+  let 'State ((
+        auction_state_128,
+        highest_bid_129,
+        st2_130,
+        expiry_131,
+        SeqMap ((m0_132, m1_133))
+      )) :=
+    (state_127) in 
+  let result_134 : (result (state_t × finalize_action_t) finalize_error_t) :=
+    @Ok (state_t × finalize_action_t) finalize_error_t (((state_127), Accept
+      )) in 
+  ifbnd negb ((auction_state_128) =.? (NotSoldYet)) : bool
+  thenbnd (bind (@Err (state_t × finalize_action_t) finalize_error_t (
+        AuctionFinalized)) (fun _ => Ok (tt)))
+  else (tt) >> (fun 'tt =>
+  let '(slot_time_135, owner_136, balance_137) :=
+    ctx_126 in 
+  ifbnd negb ((slot_time_135) >.? (expiry_131)) : bool
+  thenbnd (bind (@Err (state_t × finalize_action_t) finalize_error_t (
+        AuctionStillActive)) (fun _ => Ok (tt)))
+  else (tt) >> (fun 'tt =>
+  ifbnd (balance_137) !=.? (@repr WORDSIZE64 0) : bool
+  thenbnd (let return_action_138 : finalize_action_t :=
+      SimpleTransfer (seq_concat (seq_concat (seq_new_ (default) (usize 0)) (
+            owner_136)) (u64_to_be_bytes (highest_bid_129))) in 
+    let remaining_bid_139 : bid_remain_t :=
+      BidNone in 
+    bind (foldibnd (usize 0) to ((seq_len ((m0_132))) / (usize 32)) for (
+        auction_state_128,
+        return_action_138,
+        remaining_bid_139
+      ) >> (fun x_140 '(auction_state_128, return_action_138, remaining_bid_139
+      ) =>
+      let addr_141 : user_address_t :=
+        array_from_seq (32) (seq_slice ((m0_132)) ((x_140) * (usize 32)) (
+            usize 32)) in 
+      let amnt_142 : int64 :=
+        u64_from_be_bytes (array_from_seq (8) (seq_slice ((m1_133)) ((x_140) * (
+                usize 8)) (usize 8))) in 
+      ifbnd (amnt_142) <.? (highest_bid_129) : bool
+      then (let return_action_138 :=
+          match return_action_138 with
+          | Accept => Accept
+          | SimpleTransfer m_143 => SimpleTransfer (seq_concat (seq_concat (
+                m_143) (addr_141)) (u64_to_be_bytes (amnt_142)))
+          end in 
+        (auction_state_128, return_action_138, remaining_bid_139))
+      elsebnd(ifbnd negb ((remaining_bid_139) =.? (BidNone)) : bool
+        thenbnd (bind (@Err (state_t × finalize_action_t) finalize_error_t (
+              BidMapError)) (fun _ => Ok (tt)))
+        else (tt) >> (fun 'tt =>
+        let auction_state_128 :=
+          Sold (addr_141) in 
+        let remaining_bid_139 :=
+          BidSome (amnt_142) in 
+        Ok ((auction_state_128, return_action_138, remaining_bid_139
+          )))) >> (fun '(auction_state_128, return_action_138, remaining_bid_139
+      ) =>
+      Ok ((auction_state_128, return_action_138, remaining_bid_139))))) (fun '(
+        auction_state_128,
+        return_action_138,
+        remaining_bid_139
+      ) => let result_134 :=
+        match remaining_bid_139 with
+        | BidSome amount_144 => (if (negb ((amount_144) =.? (
+                highest_bid_129))):bool then (@Err (state_t × finalize_action_t
+            ) finalize_error_t (BidMapError)) else (@Ok (
+              state_t ×
+              finalize_action_t
+            ) finalize_error_t ((
+                State ((
+                    auction_state_128,
+                    highest_bid_129,
+                    st2_130,
+                    expiry_131,
+                    SeqMap (((m0_132), (m1_133)))
+                  )),
+                return_action_138
+              ))))
+        | BidNone => @Err (state_t × finalize_action_t) finalize_error_t (
+          BidMapError)
+        end in 
+      bind ((result_134)) (fun _ => Ok ((auction_state_128, result_134)))))
+  else ((auction_state_128, result_134)) >> (fun '(auction_state_128, result_134
+  ) =>
+  result_134))).
+
+Definition auction_test_init
+  (item_145 : public_byte_seq)
+  (time_146 : int64)
+  : bool :=
+  (fresh_state ((item_145)) (time_146)) =.? (State ((
+        NotSoldYet,
+        @repr WORDSIZE64 0,
+        (item_145),
+        time_146,
+        SeqMap ((seq_new_ (default) (usize 0), seq_new_ (default) (usize 0)))
+      ))).
+
+Theorem ensures_auction_test_init : forall result_1 (
+  item_145 : public_byte_seq) (time_146 : int64),
+@auction_test_init item_145 time_146 = result_1 ->
+result_1 = true.
+Proof. Admitted.
+QuickChick (
+  forAll g_public_byte_seq (fun item_145 : public_byte_seq =>forAll g_int64 (fun time_146 : int64 =>auction_test_init item_145 time_146))).
+
+
+Definition verify_bid
+  (item_147 : public_byte_seq)
+  (state_148 : state_t)
+  (account_149 : user_address_t)
+  (ctx_150 : context_t)
+  (amount_151 : int64)
+  (bid_map_152 : seq_map_t)
+  (highest_bid_153 : int64)
+  (time_154 : int64)
+  : (state_t × seq_map_t × bool × bool) :=
+  let t_155 : (result state_t bid_error_t) :=
+    auction_bid (ctx_150) (amount_151) ((state_148)) in 
+  let '(state_156, res_157) :=
+    match t_155 with
+    | Err e_158 => (state_148, false)
+    | Ok s_159 => (s_159, true)
+    end in 
+  let bid_map_160 : seq_map_t :=
+    match seq_map_update_entry ((bid_map_152)) (account_149) (
+      highest_bid_153) with
+    | Update (_, updated_map_161) => updated_map_161
+    end in 
+  (
+    (state_156),
+    (bid_map_160),
+    res_157,
+    ((state_156)) =.? (State ((
+          NotSoldYet,
+          highest_bid_153,
+          (item_147),
+          time_154,
+          (bid_map_160)
+        )))
+  ).
+
+Definition useraddress_from_u8 (i_162 : int8) : user_address_t :=
+  array_from_list int8 (let l :=
+      [
+        i_162;
+        i_162;
+        i_162;
+        i_162;
+        i_162;
+        i_162;
+        i_162;
+        i_162;
+        i_162;
+        i_162;
+        i_162;
+        i_162;
+        i_162;
+        i_162;
+        i_162;
+        i_162;
+        i_162;
+        i_162;
+        i_162;
+        i_162;
+        i_162;
+        i_162;
+        i_162;
+        i_162;
+        i_162;
+        i_162;
+        i_162;
+        i_162;
+        i_162;
+        i_162;
+        i_162;
+        i_162
+      ] in  l).
+
+Definition new_account
+  (time_163 : int64)
+  (i_164 : int8)
+  : (user_address_t × context_t) :=
+  let addr_165 : user_address_t :=
+    useraddress_from_u8 (i_164) in 
+  let ctx_166 : (int64 × user_address_set_t) :=
+    (time_163, UserAddressSome (addr_165)) in 
+  (addr_165, ctx_166).
+
+Definition test_auction_bid_and_finalize
+  (item_167 : public_byte_seq)
+  (time_168 : int64)
+  (input_amount_169 : int64)
+  : bool :=
+  let amount_170 : int64 :=
+    (input_amount_169) .+ (@repr WORDSIZE64 1) in 
+  let winning_amount_171 : int64 :=
+    (amount_170) .* (@repr WORDSIZE64 3) in 
+  let big_amount_172 : int64 :=
+    (amount_170) .* (@repr WORDSIZE64 5) in 
+  let bid_map_173 : seq_map_t :=
+    SeqMap ((seq_new_ (default) (usize 0), seq_new_ (default) (usize 0))) in 
+  let state_174 : state_t :=
+    fresh_state ((item_167)) (time_168) in 
+  let '(alice_175, alice_ctx_176) :=
+    new_account (time_168) (@repr WORDSIZE8 0) in 
+  let '(state_177, bid_map_178, res_0_179, result_0_180) :=
+    verify_bid ((item_167)) (state_174) (alice_175) (alice_ctx_176) (
+      amount_170) (bid_map_173) (amount_170) (time_168) in 
+  let '(state_181, bid_map_182, res_1_183, result_1_184) :=
+    verify_bid ((item_167)) (state_177) (alice_175) (alice_ctx_176) (
+      amount_170) (bid_map_178) ((amount_170) .+ (amount_170)) (time_168) in 
+  let '(bob_185, bob_ctx_186) :=
+    new_account (time_168) (@repr WORDSIZE8 1) in 
+  let '(state_187, bid_map_188, res_2_189, result_2_190) :=
+    verify_bid ((item_167)) (state_181) (bob_185) (bob_ctx_186) (
+      winning_amount_171) (bid_map_182) (winning_amount_171) (time_168) in 
+  let owner_191 : user_address_t :=
+    useraddress_from_u8 (@repr WORDSIZE8 0) in 
+  let balance_192 : int64 :=
+    @repr WORDSIZE64 100 in 
+  let ctx4_193 : (int64 × user_address_t × int64) :=
+    (time_168, owner_191, balance_192) in 
+  let finres_194 : (result (state_t × finalize_action_t) finalize_error_t) :=
+    auction_finalize (ctx4_193) ((state_187)) in 
+  let '(state_195, result_3_196) :=
+    match finres_194 with
+    | Err err_197 => ((state_187), (err_197) =.? (AuctionStillActive))
+    | Ok (state_198, _) => (state_198, false)
+    end in 
+  let '(carol_199, carol_ctx_200) :=
+    new_account (time_168) (@repr WORDSIZE8 2) in 
+  let ctx5_201 : (int64 × user_address_t × int64) :=
+    ((time_168) .+ (@repr WORDSIZE64 1), carol_199, winning_amount_171) in 
+  let finres2_202 : (result (state_t × finalize_action_t) finalize_error_t) :=
+    auction_finalize (ctx5_201) ((state_195)) in 
+  let '(state_203, result_4_204) :=
+    match finres2_202 with
+    | Err _ => ((state_195), false)
+    | Ok (state_205, action_206) => (
+      state_205,
+      (action_206) =.? (SimpleTransfer (seq_concat (seq_concat (seq_concat (
+                seq_concat (seq_new_ (default) (usize 0)) (carol_199)) (
+                u64_to_be_bytes (winning_amount_171))) (alice_175)) (
+            u64_to_be_bytes ((amount_170) .+ (amount_170)))))
+    )
+    end in 
+  let result_5_207 : bool :=
+    ((state_203)) =.? (State ((
+          Sold (bob_185),
+          winning_amount_171,
+          (item_167),
+          time_168,
+          (bid_map_188)
+        ))) in 
+  let finres3_208 : (result (state_t × finalize_action_t) finalize_error_t) :=
+    auction_finalize (ctx5_201) ((state_203)) in 
+  let '(state_209, result_6_210) :=
+    match finres3_208 with
+    | Err err_211 => (state_203, (err_211) =.? (AuctionFinalized))
+    | Ok (state_212, action_213) => (state_212, false)
+    end in 
+  let t_214 : (result state_t bid_error_t) :=
+    auction_bid (bob_ctx_186) (big_amount_172) ((state_209)) in 
+  let result_7_215 : bool :=
+    match t_214 with
+    | Err e_216 => (e_216) =.? (AuctionIsFinalized)
+    | Ok _ => false
+    end in 
+  (((((((result_0_180) && (result_1_184)) && (result_2_190)) && (
+            result_3_196)) && (result_4_204)) && (result_5_207)) && (
+      result_6_210)) && (result_7_215).
+
+Theorem ensures_test_auction_bid_and_finalize : forall result_1 (
+  item_167 : public_byte_seq) (time_168 : int64) (input_amount_169 : int64),
+@test_auction_bid_and_finalize item_167 time_168 input_amount_169 = result_1 ->
+result_1 = true.
+Proof. Admitted.
+QuickChick (
+  forAll g_public_byte_seq (fun item_167 : public_byte_seq =>forAll g_int64 (fun time_168 : int64 =>forAll g_int64 (fun input_amount_169 : int64 =>test_auction_bid_and_finalize item_167 time_168 input_amount_169)))).
+
+
